theories/common.v
@@ -1,0 +1,238 @@
+
+From iris.heap_lang Require Import lang proofmode notation.
+From Deque Require Import tick.
+
+(* Section notations *)
+Notation "⋅ x" := [x] (at level 60).
+Definition nonempty {A : Type} (x : list A) := ~(x = []).
+Notation "[3..6]" := [3; 4; 5; 6].
+Notation "[2..6]" := [2; 3; 4; 5; 6].
+Notation "[1..7]" := [1; 2; 3; 4; 5; 6; 7].
+Notation "[1..8]" := [1; 2; 3; 4; 5; 6; 7; 8].
+(* End notations *)
+
+Section assumptions.
+  Context `{!heapGS Σ}.
+
+  (* All functions in this section are assumed to run in O(1) time and space. *)
+
+  Section buffers.
+    (* Buffers will have bounded size, guaranteeing O(1) time and space complexity *)
+
+    Definition raw_buffer (o : list val) : val -> iProp Σ.
+    Admitted.
+
+    Global Instance raw_bufferPersistent o v : Persistent (raw_buffer o v).
+    Admitted.
+
+    Definition empty_buffer : val.
+    Admitted.
+
+    Axiom empty_is_buffer : ⊢ raw_buffer [] empty_buffer.
+
+    Definition bpush : val.
+    Admitted.
+
+    Property bpush_spec : forall o b x,
+      {{{ raw_buffer o b }}}
+        bpush x b
+      {{{ b', RET b'; raw_buffer (⋅x ++ o) b' }}}.
+    Admitted.
+
+    Definition bpop : val.
+    Admitted.
+
+    Property bpop_spec : forall o b x,
+      {{{ raw_buffer (⋅x ++ o) b }}}
+        bpop b
+      {{{ b', RET (x, b')%V; raw_buffer o b' }}}.
+    Admitted.
+
+    Definition binject : val.
+    Admitted.
+
+    Property binject_spec : forall o b x,
+      {{{ raw_buffer o b }}}
+        binject x b
+      {{{ b', RET b'; raw_buffer (o ++ ⋅x) b' }}}.
+    Admitted.
+
+    Definition beject : val.
+    Admitted.
+
+    Property beject_spec : forall o b x,
+      {{{ raw_buffer (o ++ ⋅x) b }}}
+        beject b
+      {{{ b', RET (x, b')%V; raw_buffer o b' }}}.
+    Admitted.
+
+    Definition bsize : val.
+    Admitted.
+
+    Property bsize_spec : forall o b,
+      {{{ raw_buffer o b }}}
+        bsize b
+      {{{ RET #(length o); emp }}}.
+    Admitted.
+
+    Definition partition_buffer_left : val.
+    Admitted.
+
+    Property partition_buffer_left_spec : forall o b,
+      {{{ raw_buffer o b ∗ ⌜ length o ∈ [2..6] ⌝ }}}
+        partition_buffer_left b
+      {{{ b1 b2, RET (b1, b2)%V;
+        ∃ o1 o2, raw_buffer o1 b1 ∗ raw_buffer o2 b2 ∗
+          ⌜ length o1 ∈ [2; 3] ∧ length o2 ∈ [0; 2; 3] ∧ o1 ++ o2 = o ⌝ }}}.
+    Admitted.
+
+    Definition partition_buffer_right : val.
+    Admitted.
+
+    Property partition_buffer_right_spec : forall o b,
+      {{{ raw_buffer o b ∗ ⌜ length o ∈ [2..6] ⌝ }}}
+        partition_buffer_right b
+      {{{ b1 b2, RET (b1, b2)%V;
+        ∃ o1 o2, raw_buffer o1 b1 ∗ raw_buffer o2 b2 ∗
+          ⌜ length o1 ∈ [0; 2; 3] ∧ length o2 ∈ [2; 3] ∧ o1 ++ o2 = o ⌝ }}}.
+    Admitted.
+
+    (* NOTE(Juliette): basically [fold_right push] and [fold_left inject] *)
+    Definition push_whole_buffer : val. Admitted.
+    Definition inject_whole_buffer : val. Admitted.
+
+  End buffers.
+
+End assumptions.
+
+Hint Resolve elem_of_list_here : find_in_list.
+Hint Resolve elem_of_list_further : find_in_list.
+
+Ltac find := eauto with find_in_list.
+
+Section configurations.
+  (* This section describes buffer configurations and potentials *)
+
+  (* Triple configuration: first and last are [2;3] *)
+  Inductive triple_configuration : nat -> nat -> nat -> Prop :=
+    | left_leaning : forall x y, x ∈ [2; 3] -> y ∈ [0; 2; 3] -> triple_configuration x 0 y
+    | has_child : forall x o y, x ∈ [2; 3] -> o > 0 -> y ∈ [2; 3] -> triple_configuration x o y.
+
+  (* Five-tuple configuration matching OCaml invariants *)
+  Inductive five_tuple_configuration : nat -> nat -> nat -> nat -> nat -> Prop :=
+    | suffix_only : forall s, s ∈ [1..8] -> five_tuple_configuration 0 0 0 0 s
+    | has_middle : forall p ld rd s, p ∈ [3..6] -> s ∈ [3..6] -> five_tuple_configuration p ld 2 rd s.
+
+
+  Inductive colour : Set :=
+    | green | red | very_red.
+
+  Definition buffer_colour : nat -> colour :=
+    λ n,
+    match n with
+    | 8 => very_red
+    | 3 | 6 => red
+    | _ => green
+    end.
+
+End configurations.
+
+(* Potential associated with the first and last argument of the five-tuple configuration *)
+Notation "pre ⋄ suf" :=
+  (match buffer_colour pre, buffer_colour suf with
+  | _, very_red | red, red => 3
+  | red, green | green, red => 1
+  | _, _ => 0
+  end) (at level 60).
+
+Section algorithms.
+
+  Context `{!heapGS Σ}.
+
+  Let empty := NONEV.
+
+  Example singleton_deque : val :=
+    λ: "x", SOME (ref (empty_buffer, NONEV, empty_buffer, NONEV, bpush "x" empty_buffer)%E).
+
+  Notation "'let:2' ( x , y ) := u 'in' v"
+  := (let: "TMP2" := u in
+      let: x := Fst "TMP2" in
+      let: y := Snd "TMP2" in
+      v)%E
+     (at level 190, x,y at next level, u at next level, v at next level, only parsing).
+
+  Notation "'let:5' ( v , w , x , y , z ) := U 'in' V"
+    := (let: "TMP5" := U in
+        let:2 ("TMP5", z) := "TMP5" in
+        let:2 ("TMP5", y) := "TMP5" in
+        let:2 ("TMP5", x) := "TMP5" in
+        let:2 (v, w) := "TMP5" in
+        V)%E
+      (at level 190, v,w,x,y,z at next level, U at next level, V at next level, only parsing).
+
+  Definition push : val :=
+    rec: "push" "x" "d" :=
+    tick #();;
+    match: "d" with
+      NONE => singleton_deque "x"
+    | SOME "r" =>
+      let:5 ("prefix", "left_deque", "middle", "right_deque", "suffix") := !"r" in
+      if: bsize "middle" = #0%nat then (
+        (* suffix-only *)
+        if: bsize "suffix" = #8%nat then (
+          let:2 ("x1", "suffix") := bpop "suffix" in
+          let:2 ("x2", "suffix") := bpop "suffix" in
+          let:2 ("x3", "suffix") := bpop "suffix" in
+          let: "prefix" := bpush "x1" (bpush "x2" (bpush "x3" empty_buffer)) in
+          let:2 ("x4", "suffix") := bpop "suffix" in
+          let:2 ("x5", "suffix") := bpop "suffix" in
+          let: "middle" := bpush "x4" (bpush "x5" empty_buffer) in
+          "r" <- ( "prefix", empty, "middle", empty, "suffix" );;
+          SOME (ref (bpush "x" "prefix", empty, "middle", empty, "suffix"))
+        ) else (
+          "r" <- ("prefix", "left_deque", "middle", "right_deque", "suffix");;
+          SOME (ref ("prefix", "left_deque", "middle", "right_deque", bpush "x" "suffix"))
+        )
+      ) else (
+        (* normal mode *)
+        if: bsize "prefix" = #6%nat then (
+          let:2 ("prefix", "x6") := beject "prefix" in
+          let:2 ("prefix", "x5") := beject "prefix" in
+          let: "prefix'" := bpush "x5" (bpush "x6" empty_buffer) in
+          let: "left_deque" := "push" ("prefix'", empty, empty_buffer) "left_deque" in
+          "r" <- ( "prefix", "left_deque", "middle", "right_deque", "suffix" );;
+          SOME (ref (bpush "x" "prefix", "left_deque", "middle", "right_deque", "suffix"))
+        ) else
+          "r" <- ("prefix", "left_deque", "middle", "right_deque", "suffix");;
+          SOME (ref (bpush "x" "prefix", "left_deque", "middle", "right_deque", "suffix"))
+      )
+    end.
+
+  Corollary inject : val. Admitted.
+
+  Definition dconcat : val :=
+    λ: "d1" "d2",
+    tick #();;
+    match: "d1" with NONE => "d2"
+    | SOME "r1" =>
+    match: "d2" with NONE => "d1"
+    | SOME "r2" =>
+    let:5 ("pr1", "ld1", "md1", "rd1", "sf1") := !"r1" in
+    if: bsize "md1" = #0%nat then push_whole_buffer push "sf1" "d2" else
+    let:5 ("pr2", "ld2", "md2", "rd2", "sf2") := !"r2" in
+    if: bsize "md2" = #0%nat then inject_whole_buffer inject "d1" "sf2" else
+    let:2 ("y", "pr2'") := bpop "pr2" in
+    let:2 ("sf1'", "x") := beject "sf1" in
+    let: "middle" := bpush "x" (bpush "y" empty_buffer) in
+    let:2 ("s1'", "s1''") := partition_buffer_left "sf1'" in
+    let: "ld1'" := inject "ld1" ("md1", "rd1", "s1'") in
+    let: "ld1''" := if: bsize "s1''" = #0%nat then "ld1'"
+      else inject "ld1'" ("s1''", empty, empty_buffer) in
+    let:2 ("p2'", "p2''") := partition_buffer_right "pr2'" in
+    let: "rd2'" := push ("p2''", "ld2", "md2") "rd2" in
+    let: "rd2''" := if: bsize "p2'" = #0%nat then "rd2'"
+      else push ("p2'", empty, empty_buffer) "rd2'" in
+    SOME (ref ("pr1", "ld1''", "middle", "rd2''", "sf2"))
+    end end.
+
+End algorithms.
