theories/counter.v
@@ -1,0 +1,41 @@
+
+From iris.heap_lang Require Import lang proofmode notation.
+
+Section counter.
+  Context `{!heapGS Σ}.
+
+  (* Program Counter *)
+  Local Parameter ℓ : loc.
+
+  Definition CounterExact (n : Z) : iProp Σ := ℓ ↦ #n.
+  Definition Counter (n : Z) : iProp Σ := ∃ k, ⌜ (k <= n)%Z ⌝ ∗ CounterExact k.
+
+  Definition tick_up : val :=
+    λ: "", (#ℓ <- !#ℓ + #1)%E.
+
+  Theorem tick_up_spec : forall n : nat,
+    {{{ Counter n }}} tick_up #() {{{ RET #(); Counter (n + 1) }}}.
+  Proof.
+    iIntros (n ψ) "(%k & %Hlt & Hℓ) Hψ".
+    rewrite /tick_up. wp_pures.
+    wp_load.
+    wp_pures.
+    wp_store.
+    iApply "Hψ".
+    iExists (k+1)%Z.
+    iFrame.
+    iPureIntro.
+    lia.
+  Qed.
+
+  Theorem Counter_single : forall n m, Counter n ∗ Counter m ⊢ False.
+  Proof.
+    iIntros (n m) "[(%k1 & _ & H1) (%k2 & _ & H2)]".
+    rewrite /CounterExact.
+    iCombine "H1 H2" gives "[%H _]".
+    contradiction.
+  Qed.
+End counter.
+
+Opaque CounterExact.
+Opaque tick_up.
