theories/deque_safe.v
@@ -1,0 +1,982 @@
+From iris.heap_lang Require Import lang proofmode notation.
+From iris.bi Require Import derived_laws.
+
+From Coq Require Import List.
+Import ListNotations.
+
+From AAC_tactics Require Import AAC.
+From AAC_tactics Require Import Instances.
+Import Instances.Lists.
+
+From Deque Require Import common tick shared_ref.
+
+Section safe_deques.
+  (* This section describes the structure used for the proof of the time-complexity bounds *)
+
+  Context `{!heapGS Σ} `{!na_invG Σ}.
+
+  Let isDequeType := nat -d> list val -d> val -d> iProp Σ.
+
+  (* Buffer unwinding: abstract content depends on level *)
+  Definition bufferPre (size : nat) : isDequeType -d> isDequeType := (
+  λ self_triple n content buf,
+    match n with
+    | 0 => raw_buffer content buf ∗ ⌜ length content = size ⌝
+    | S n =>
+        ∃ (triples : list val) (triple_contents : list (list val)),
+          raw_buffer triples buf ∗
+          ⌜ content = List.concat triple_contents ∧ length triples = size ⌝ ∗
+          [∗ list] tri; c ∈ triples; triple_contents, ▷ self_triple n c tri
+    end
+  )%I.
+
+  Global Instance bufferPreContractive size : Contractive (bufferPre size).
+  Proof.
+    rewrite /bufferPre.
+    intros k f1 f2 Hdist n c b.
+    repeat (f_contractive || f_equiv).
+    apply (Hdist _ _ _).
+  Qed.
+
+  Definition five_tuple_potential : nat -> nat -> iProp Σ :=
+    λ pre suf, ⏱ (pre ⋄ suf).
+
+  Let fFiveTuple (triple_pred : isDequeType) (deque_pred : isDequeType) : isDequeType := (
+    λ n o d, ∃ (pr ld md rd sf : val)
+      (pr_content left_content md_content right_content sf_content : list val)
+      (kPr kMd kSf : nat),
+      ⌜ d = (pr, ld, md, rd, sf)%V ⌝ ∗
+      ⌜ five_tuple_configuration kPr (length left_content) kMd (length right_content) kSf ⌝ ∗
+      bufferPre kPr triple_pred n pr_content pr ∗
+      deque_pred (S n) left_content ld ∗
+      bufferPre kMd triple_pred n md_content md ∗
+      deque_pred (S n) right_content rd ∗
+      bufferPre kSf triple_pred n sf_content sf ∗
+      ⌜ o = pr_content ++ left_content ++ md_content ++ right_content ++ sf_content ⌝
+  )%I.
+
+  (* Define the mutual fixpoint functions *)
+  Let fDeque (triple_pred : isDequeType) (deque_pred : isDequeType) : isDequeType := (
+    λ n o d,
+      (⌜ d = NONEV ∧ o = [] ⌝) ∨
+      (∃ ℓ : loc, ⌜ d = SOMEV #ℓ ⌝ ∗
+        ℓ ⤇ fFiveTuple triple_pred deque_pred n o)
+  )%I.
+
+  Let fTriple (triple_pred : isDequeType) (deque_pred : isDequeType) : isDequeType := (
+    λ n o t,
+      ∃ (fst ch lst : val)
+        (fst_content child_content lst_content : list val)
+        (kFst kLst : nat),
+        ⌜ triple_configuration kFst (length child_content) kLst ⌝ ∗
+        ⌜ t = (fst, ch, lst)%V ⌝ ∗
+        bufferPre kFst triple_pred n fst_content fst ∗
+        deque_pred (S n) child_content ch ∗
+        bufferPre kLst triple_pred n lst_content lst ∗
+        ⌜ o = fst_content ++ child_content ++ lst_content ⌝
+  )%I.
+
+  (* Prove contractivity *)
+  Local Instance fDeque_contractive :
+    ∀ n, Proper (dist_later n ==> dist_later n ==> dist n) fDeque.
+  Proof.
+    intros k deque1 deque2 Hdist_cad triple1 triple2 Hdist_tri.
+    intros n o d.
+    rewrite /fDeque.
+    do 4 (f_contractive || f_equiv).
+    rewrite /csref.
+    do 4 (f_contractive || f_equiv).
+    rewrite /fFiveTuple.
+    do 29 (f_contractive || f_equiv). apply bufferPreContractive, dist_dist_later, Hdist_cad.
+    f_equiv. by apply (Hdist_tri _ _ _).
+    f_equiv. by apply bufferPreContractive, dist_dist_later, Hdist_cad.
+    f_equiv. apply (Hdist_tri _ _ _).
+    f_equiv. apply bufferPreContractive, dist_dist_later, Hdist_cad.
+  Qed.
+
+  Local Instance fTriple_contractive :
+    ∀ n, Proper (dist_later n ==> dist n ==> dist n) fTriple.
+  Proof.
+    intros k deque1 deque2 Hdist_cad triple1 triple2 Hdist_tri.
+    intros n o t.
+    rewrite /fTriple.
+    do 19 (f_contractive || f_equiv).
+    - by apply bufferPreContractive.
+    - f_equiv. by apply (Hdist_tri _ _ _).
+      f_equiv. by apply bufferPreContractive.
+  Qed.
+
+  Definition triple := fixpoint_A fTriple fDeque.
+  Definition isDeque := fixpoint_B fTriple fDeque.
+  Definition fiveTuple := fFiveTuple triple isDeque.
+  Definition isElement n o e := match n with 0 => ⌜ o = [e] ⌝%I | S n => triple n o e end.
+  Definition buffer size := bufferPre size triple.
+  Definition IsDeque o d := isDeque 0 o d.
+
+  (* Unfolding lemmas come directly from the fixpoint theory *)
+  Lemma isDeque_unfold n o d :
+    isDeque n o d ⊣⊢ fDeque triple isDeque n o d.
+  Proof.
+    symmetry.
+    apply (fixpoint_B_unfold fTriple fDeque _ _ _).
+  Qed.
+
+  Lemma triple_unfold n o t :
+    triple n o t ⊣⊢ fTriple triple isDeque n o t.
+  Proof.
+    symmetry.
+    apply (fixpoint_A_unfold fTriple fDeque _ _ _).
+  Qed.
+
+  (* Persistence instances *)
+  Global Instance bufferPersistent s ϕ n b c :
+    (∀ n o d, Persistent (ϕ n o d)) → Persistent (bufferPre s ϕ n b c).
+  Proof.
+    intros HPers.
+    rewrite /bufferPre.
+    destruct n; apply _.
+  Qed.
+
+  Global Instance isDequePersistent n o d : Persistent (isDeque n o d).
+  Proof.
+    rewrite isDeque_unfold /fDeque.
+    apply _.
+  Qed.
+
+  Global Instance triplePersistent n o t : Persistent (triple n o t).
+  Proof.
+    rewrite /triple /fixpoint_A /ofe.fixpoint_AB.
+    revert n o t. apply fixpoint_ind.
+    - intros f1 f2 H P n o t. rewrite -(H _ _ _) //.
+    - exists (λ _ _ _, emp)%I. apply _.
+    - intros.
+      rewrite /ofe.fixpoint_AA /fTriple /ofe.fixpoint_AB.
+      assert (forall a b, Persistent (fixpoint (fDeque x) (S n) a b)); [| apply _].
+      intros. apply fixpoint_ind.
+        + intros f1 f2 H' P'. rewrite -(H' _ _ _) //.
+        + exists (λ _ _ _, emp)%I. apply _.
+        + apply _.
+        + apply bi.limit_preserving_Persistent.
+          intros k f1 f2 Hdist. apply (Hdist _ _ _).
+    - apply limit_preserving_forall => n.
+      apply limit_preserving_forall => o.
+      apply limit_preserving_forall => t.
+      apply bi.limit_preserving_Persistent.
+      intros k f1 f2 Hdist. apply (Hdist _ _ _).
+  Qed.
+
+  Global Instance fiveTuplePersistent n o d : Persistent (fiveTuple n o d).
+  Proof.
+    apply _.
+  Qed.
+
+  Global Instance isElementPersistent n o e : Persistent (isElement n o e).
+  Proof.
+    destruct n; apply _.
+  Qed.
+
+End safe_deques.
+
+Section proofs.
+
+  Context `{!heapGS Σ} `{!na_invG Σ}.
+
+  (* Disregard time analysis completely. *)
+  Axiom tick_spec : {{{ emp }}} tick #() {{{ RET #(); emp }}}.
+
+  Ltac ℓisDeque ℓ := rewrite !isDeque_unfold; iRight; iExists ℓ; iSplitR; [done |].
+
+  Ltac isEmptyDeque := rewrite !isDeque_unfold; iLeft; iPureIntro; done.
+
+  Lemma bool_decide_code_true (a : nat) (b : nat) : bool_decide (a = b) = true -> bool_decide (#a = #b) = true.
+  Proof.
+    intro.
+    apply bool_decide_eq_true_1 in H.
+    by apply bool_decide_eq_true_2, f_equal, f_equal, f_equal.
+  Qed.
+
+  Lemma bool_decide_code_false (a : nat) (b : nat) : bool_decide (a = b) = false -> bool_decide (#a = #b) = false.
+  Proof.
+    intro.
+    apply bool_decide_eq_false_1 in H.
+    apply bool_decide_eq_false_2.
+    intro. apply H.
+    inversion H0.
+    by apply Nat2Z.inj'.
+  Qed.
+
+  Example singleton_deque_spec : forall x : val,
+    {{{ emp }}} singleton_deque x {{{ d, RET d; IsDeque (⋅x) d }}}.
+  Proof.
+    iIntros (x Φ) "_ Hψ".
+    rewrite /singleton_deque. wp_pures.
+    wp_bind (bpush _ _)%E.
+    wp_apply (bpush_spec) as "%b #Hb".
+      { iApply empty_is_buffer. }
+    wp_pures.
+    wp_bind (ref _)%E.
+    wp_apply (csref_alloc (fiveTuple 0 (⋅ x))) as "%ℓ Hℓ".
+      { rewrite /fiveTuple.
+        iExists empty_buffer, empty, empty_buffer, empty, b,
+                []          , []   , []          , []    , (⋅x),
+                0, 0, 1.
+        rewrite //=.
+        iSplitL. rewrite //.
+        iSplitL. iPureIntro. constructor. by auto with find_in_list.
+        iSplitL. iSplitL. iApply empty_is_buffer. done.
+        iSplitL. isEmptyDeque.
+        iSplitL. iSplitL. iApply empty_is_buffer. done.
+        iSplitL. isEmptyDeque.
+        iFrame "#". done.
+      }
+    wp_pures.
+    iApply "Hψ".
+    iModIntro.
+    rewrite /IsDeque. ℓisDeque ℓ.
+    done.
+  Qed.
+
+  Ltac isEmptyBufferAtDepth depth :=
+  destruct depth;
+  [ iSplitL; [by iApply empty_is_buffer | rewrite //]
+  | iExists [], []; iSplitL; try iSplitL; rewrite //; by iApply empty_is_buffer ].
+
+  Lemma bsize_better_spec k n o b :
+    {{{ buffer k n o b }}}
+      bsize b
+    {{{ RET #k; True }}}.
+  Proof.
+    iIntros (ψ) "Hb Hψ".
+    destruct n.
+    - iDestruct "Hb" as "[Hb <-]".
+      by iApply (bsize_spec with "Hb").
+    - iDestruct "Hb" as "(%tr & %trC & Hb & (_ & %Heq) & _)".
+      iApply (bsize_spec with "Hb").
+      by subst.
+  Qed.
+
+  Lemma empty_is_buffer_at : forall depth, ⊢ buffer 0 depth [] empty_buffer.
+  Proof.
+    destruct depth.
+    - iSplitR; [ by iApply empty_is_buffer | done ].
+    - iExists [], [].
+      iSplitR; [ by iApply empty_is_buffer |].
+      iSplitR; done.
+  Qed.
+
+  Lemma singleton_deque_better : forall depth x oX b, isElement depth oX x -∗ raw_buffer (⋅x) b -∗ fiveTuple depth oX (empty_buffer, NONEV, empty_buffer, NONEV, b)%V.
+  Proof.
+    iIntros (depth x oX b) "Hx #Hb".
+    iExists empty_buffer, empty, empty_buffer, empty, b,
+            []          , []   , []          , []   , oX,
+            0, 0, 1.
+    rewrite /=.
+    iSplitR. rewrite //.
+    iSplitR. iPureIntro. constructor. auto with find_in_list.
+    iSplitR. isEmptyBufferAtDepth depth.
+    iSplitR. isEmptyDeque.
+    iSplitR. isEmptyBufferAtDepth depth.
+    iSplitR. isEmptyDeque.
+    iSplitL; [| done].
+    rewrite /bufferPre.
+    destruct depth.
+    - iDestruct "Hx" as "->"; iSplitL; rewrite //.
+    - rewrite /isElement.
+      iExists [x], [oX].
+      iSplitR. done.
+      iSplitR. iSplitR. iPureIntro. rewrite /=. by aac_reflexivity.
+      iPureIntro. split; rewrite //=; by aac_reflexivity.
+      rewrite /=; iSplitL; done.
+  Qed.
+
+  Lemma empty_buffer_is_empty : forall n b o, buffer 0 n o b ⊢ ⌜ o = [] ⌝.
+  Proof.
+    destruct n; iIntros (b o) "H".
+    - iDestruct "H" as "[_ %Heq]". iPureIntro; by apply nil_length_inv.
+    - iDestruct "H" as "(%t & %c & _ & (%Hc & %Heq) & H)".
+      iDestruct (big_sepL2_length with "H") as "%Hl".
+      iPureIntro.
+      rewrite Hc.
+      rewrite Hl in Heq.
+      apply nil_length_inv in Heq.
+      by rewrite Heq //.
+  Qed.
+
+  Lemma push_buffer_element_spec x b : forall n o oX size,
+    {{{ isElement n oX x ∗ buffer size n o b }}}
+      bpush x b
+    {{{ b', RET b'; buffer (S size) n (oX ++ o) b' }}}.
+  Proof.
+    destruct n; iIntros (o oX size ψ) "[Hx Hb] Hψ".
+    - iCombine "Hx Hb" as "[-> [Hb %sEqL]]".
+      wp_apply (bpush_spec with "Hb") as "%b' Hb'".
+      iApply "Hψ".
+      iSplitL. done.
+      iPureIntro. simpl; auto.
+    - rewrite /isElement.
+      iDestruct "Hb" as "(%triples & %triples_content & Hb & [%Ho %lenEqSz] & areTriples)".
+      wp_apply (bpush_spec with "Hb") as "%b' Hb'".
+      iApply "Hψ".
+      rewrite /buffer /bufferPre.
+      iExists (⋅ x ++ triples), (⋅ oX ++ triples_content).
+      iFrame. iSplitR.
+      + iPureIntro; split.
+        * rewrite /= Ho //.
+        * rewrite /= lenEqSz //.
+      + iSplitR. done.
+        iApply (big_sepL2_mono with "areTriples").
+        intros. iIntros "t". by iNext.
+  Qed.
+
+  Corollary inject_buffer_element_spec x b : forall n o oX size,
+    {{{ isElement n oX x ∗ buffer size n o b }}}
+      binject x b
+    {{{ b', RET b'; buffer (S size) n (o ++ oX) b' }}}.
+  Admitted.
+
+  Lemma pop_buffer_element_spec b : forall n o size,
+    {{{ buffer (S size) n o b }}}
+      bpop b
+    {{{ x b', RET (x, b'); ∃ oX o', buffer size n o' b' ∗ ⌜ o = oX ++ o' ⌝ ∗ isElement n oX x }}}.
+  Proof.
+    destruct n; iIntros (o size ψ) "Hb Hψ".
+    - iDestruct "Hb" as "[Hb %sEqL]".
+      destruct o. by inversion sEqL.
+      wp_apply (bpop_spec with "Hb") as "%b' Hb'".
+      iApply "Hψ".
+      iExists (⋅ v).
+      iFrame. iSplit; iPureIntro.
+      + by inversion sEqL.
+      + auto.
+    - iDestruct "Hb" as "(%triples & %triples_content & Hb & [%Ho %lenEqSz] & areTriples)".
+      destruct triples. by inversion lenEqSz.
+      iDestruct (big_sepL2_length with "areTriples") as "%Hlen".
+      destruct triples_content. by rewrite lenEqSz // in Hlen.
+      wp_apply (bpop_spec with "Hb") as "%b' Hb'".
+      iApply "Hψ".
+      iDestruct (big_sepL2_cons with "areTriples") as "[tri Hrest]".
+      iExists l, (List.concat triples_content).
+      iSplitL "Hb' Hrest".
+      + iExists triples, triples_content.
+        iSplitL "Hb'". done.
+        iSplitR.
+        * iPureIntro; split; [trivial |].
+          by inversion lenEqSz.
+        * iApply (big_sepL2_mono with "Hrest").
+          intros. iIntros "t". by iNext.
+      + iSplitR.
+        * iPureIntro. by rewrite Ho //.
+        * done.
+  Qed.
+
+   Corollary eject_buffer_element_spec b : forall n o size,
+    {{{ buffer (S size) n o b }}}
+      beject b
+    {{{ b' x, RET (b', x); ∃ oX o', buffer size n o' b' ∗ ⌜ o = o' ++ oX ⌝ ∗ isElement n oX x }}}.
+  Admitted.
+
+  Ltac solve_no_middle Heq H H1 :=
+  iSplitR; [done |];
+  iSplitR; [iPureIntro; constructor; auto with find_in_list |];
+  iSplitR; [trivial |];
+  iSplitR; [isEmptyDeque |];
+  iSplitR; [trivial |];
+  iSplitR; [isEmptyDeque |];
+  iSplitR; [trivial |];
+  inversion cfg;
+  [ rewrite Heq;
+    symmetry in H, H1;
+    iDestruct (empty_buffer_is_empty with "Hpr") as "->";
+    iDestruct (empty_buffer_is_empty with "Hmd") as "->";
+    rewrite (nil_length_inv _ H);
+    rewrite (nil_length_inv _ H1);
+    iPureIntro;
+    aac_reflexivity
+  | inversion H0; inversion H8; inversion H12; inversion H16; inversion H20
+  ].
+
+  Ltac invert_all_in :=
+  repeat match goal with
+  | H : _ ∈ _ |- _ =>
+    first
+    [ inversion H; clear H; auto 10 with find_in_list
+    | inversion H; clear H; [ by contradiction |]
+    | by inversion H
+    ];
+    try contradiction
+  end.
+
+  Notation time_for_push := 7.
+
+  Lemma push_spec_helper oD oX x d : forall depth,
+    {{{ isDeque depth oD d ∗ isElement depth oX x }}}
+      push x d
+    {{{ d', RET d'; isDeque depth (oX ++ oD) d'}}}.
+  Proof.
+    iLöb as "iH" forall (x d oX oD).
+    iIntros (depth ψ) "(Hd & #Hx) Hψ".
+    iAssert emp%I as "ι". done. (* time cheat *)
+    rewrite /push.
+    wp_pures.
+    wp_apply (tick_spec with "ι") as "_".
+    wp_pures.
+    rewrite {1} isDeque_unfold.
+    iDestruct "Hd" as "[[-> ->] | (%ℓ & -> & #Hℓ)]".
+    - wp_pures.
+      rewrite /singleton_deque. wp_pures.
+      wp_apply bpush_spec as "%b #Hb".
+        { iApply empty_is_buffer. }
+      wp_pures.
+      wp_bind (ref _)%E.
+      wp_apply (csref_alloc (fiveTuple depth oX) with "[Hx]") as "%ℓ #Hℓ".
+      + rewrite app_nil_r. by iApply (singleton_deque_better with "Hx").
+      + wp_pures.
+        iApply "Hψ".
+        iFrame.
+        ℓisDeque ℓ. iModIntro. rewrite !app_nil_r //.
+    - wp_pures.
+      wp_apply (csref_load with "Hℓ") as "%d #πd".
+      wp_pures.
+      iCombine "πd πd" as
+        "[#Hd (%pr & %ld & %md & %rd & %sf & %prC & %ldC & %mdC & %rdC & %sfC
+          & %kPr & %kMd & %kSf & -> & %cfg
+          & #Hpr & #Hld & #Hmd & #Hrd & #Hsf & %Heq)]".
+      wp_pures.
+      wp_bind (if: _ then _ else _)%E.
+      wp_apply (bsize_better_spec with "Hmd") as "_".
+      wp_pures.
+      destruct (bool_decide (kMd = 0)) eqn:?.
+      + apply bool_decide_eq_true_1 in Heqb as Heqmd.
+        apply bool_decide_code_true in Heqb as ->.
+        wp_pures.
+        wp_bind (if: _ then _ else _)%E.
+        wp_apply (bsize_better_spec with "Hsf") as "_".
+        wp_pures.
+        destruct (bool_decide (kSf = 8)) eqn:?.
+        * apply bool_decide_eq_true_1 in Heqb as ->.
+          wp_pures.
+          wp_apply (pop_buffer_element_spec with "Hsf") as "%x1 %b1 (%oX1 & %o1 & Hsf' & -> & Hx1)".
+          wp_pures.
+          wp_apply (pop_buffer_element_spec with "Hsf'") as "%x2 %b2 (%oX2 & %o2 & Hsf' & -> & Hx2)".
+          wp_pures.
+          wp_apply (pop_buffer_element_spec with "Hsf'") as "%x3 %b3 (%oX3 & %o3 & Hsf' & -> & Hx3)".
+          wp_pures.
+          wp_apply (push_buffer_element_spec with "[Hx3]") as "%bp3 Hbp".
+            { iFrame. rewrite Heqmd. by iApply empty_is_buffer_at. }
+          wp_apply (push_buffer_element_spec with "[Hbp Hx2]") as "%bp2 Hbp". by iFrame.
+          wp_apply (push_buffer_element_spec with "[Hbp Hx1]") as "%pr' #Hpr'". by iFrame.
+          wp_pures.
+          wp_apply (pop_buffer_element_spec with "Hsf'") as "%x4 %b4 (%oX4 & %o4 & Hsf' & -> & Hx4)".
+          wp_pures.
+          wp_apply (pop_buffer_element_spec with "Hsf'") as "%x5 %sf' (%oX5 & %o5 & #Hsf' & -> & Hx5)".
+          wp_pures.
+          wp_apply (push_buffer_element_spec with "[Hx5]") as "%bp5 Hbm".
+            { iFrame. by iApply empty_is_buffer_at. }
+          wp_apply (push_buffer_element_spec with "[Hbm Hx4]") as "%md' #Hmd'". by iFrame.
+          wp_pures.
+          rewrite !app_nil_r Heqmd.
+          wp_bind (#ℓ <- _)%E.
+          wp_apply (csref_store with "[Hℓ]") as "_".
+          {
+            iSplitR. iExact "Hℓ".
+            iExists pr', empty, md', empty, sf',
+              (oX1 ++ oX2 ++ oX3), [], (oX4 ++ oX5), [], o5,
+              3, 2, 3.
+            solve_no_middle Heq H H1.
+          }
+          wp_pures.
+          wp_bind (bpush _ _)%E.
+          iDestruct "Hx" as "#Hx".
+          wp_apply (push_buffer_element_spec with "[Hpr' Hx]") as "%pr'' #Hpr''". by iFrame "#".
+          wp_pures.
+          wp_bind (ref _)%E.
+          wp_apply (csref_alloc (fiveTuple depth (oX ++ oD)) with "[Hx ι]") as "%ℓ' #Hℓ'".
+          -- iExists pr'', empty, md', empty, sf',
+              (oX ++ oX1 ++ oX2 ++ oX3), [], (oX4 ++ oX5), [], o5,
+              4, 2, 3.
+            solve_no_middle Heq H H1.
+          -- wp_pures.
+            iApply "Hψ".
+            iFrame.
+            ℓisDeque ℓ'.
+            iExact "Hℓ'".
+        * apply bool_decide_eq_false_1 in Heqb as sfNotFull.
+          apply bool_decide_code_false in Heqb as ->.
+          wp_pures.
+          wp_bind (#ℓ <- _)%E.
+          wp_apply (csref_store with "[Hℓ]") as "_".
+          {
+            iSplitR. iExact "Hℓ".
+            iFrame. iExact "Hd".
+          }
+          wp_pures.
+          wp_apply (push_buffer_element_spec with "[Hsf Hx]") as "%sf' #Hsf'". by iFrame "#".
+          wp_pures.
+          wp_apply (csref_alloc (fiveTuple depth (oX ++ oD)) with "[Hx ι]") as "%ℓ' #Hℓ'".
+          -- iExists pr, ld, md, rd, sf',
+              [], [], [], [], (oX ++ oD),
+              0, 0, (S kSf).
+            inversion cfg; [| exfalso; lia ].
+            iDestruct (empty_buffer_is_empty with "Hpr") as "->".
+            iDestruct (empty_buffer_is_empty with "Hmd") as "->".
+            symmetry in H; rewrite (nil_length_inv _ H) in Heq |- *.
+            symmetry in H1; rewrite (nil_length_inv _ H1) in Heq |- *.
+            iSplitR; [ done |].
+            iSplitR; [ iPureIntro; constructor; invert_all_in |].
+            do 4 (iSplitR; [by trivial |]).
+            aac_normalise in Heq.
+            rewrite Heq.
+            iSplitR; [ done |].
+            iPureIntro; aac_reflexivity.
+          -- wp_pures.
+            iApply "Hψ".
+            iFrame.
+            ℓisDeque ℓ'.
+            iExact "Hℓ'".
+      + apply bool_decide_eq_false_1 in Heqb as Heqmd.
+        apply bool_decide_code_false in Heqb as Heqmd2.
+        rewrite Heqmd2.
+        wp_pures.
+        wp_apply (bsize_better_spec with "Hpr") as "_".
+        wp_pures.
+        destruct (bool_decide (kPr = 6)) eqn:?.
+        * apply bool_decide_eq_true_1 in Heqb0 as ->.
+          wp_pures.
+          wp_apply (eject_buffer_element_spec with "Hpr") as "%b6 %x6 (%oX6 & %o6 & Hpr' & -> & Hx6)".
+          wp_pures.
+          wp_apply (eject_buffer_element_spec with "Hpr'") as "%pr2 %x5 (%oX5 & %o5 & #Hpr2 & -> & Hx5)".
+          wp_pures.
+          wp_apply (push_buffer_element_spec with "[Hx6]") as "%bs6 Hbp".
+            { iFrame. by iApply empty_is_buffer_at. }
+          wp_apply (push_buffer_element_spec with "[Hbp Hx5]") as "%pr' #Hpr'". by iFrame.
+          do 4 wp_pure.
+          iSpecialize ("iH" $! (pr', NONEV, empty_buffer)%V ld (oX5 ++ oX6) ldC (S depth)).
+          wp_apply "iH" as "%ld' #Hld'"; iClear "iH". {
+            iFrame "#".
+            rewrite /isElement triple_unfold !app_nil_r.
+            iFrame.
+            iExists pr', NONEV, empty_buffer,
+              (oX5 ++ oX6), [], [],
+              2, 0.
+            iSplitR. { iPureIntro; eapply left_leaning; auto with find_in_list.  }
+            iSplitR. done.
+            iSplitR. done.
+            iSplitR. isEmptyDeque.
+            iSplitR. iApply empty_is_buffer_at.
+            iPureIntro; aac_reflexivity.
+          }
+          wp_pures.
+          wp_bind (#ℓ <- _)%E.
+          inversion cfg.
+          wp_apply (csref_store with "[Hℓ]") as "_".
+          {
+            iSplitR. iExact "Hℓ".
+            iExists pr2, ld', md, rd, sf,
+              o5, ((oX5 ++ oX6) ++ ldC), mdC, rdC, sfC,
+              4, 2, kSf.
+            iFrame "#".
+            iSplitR. done.
+            iSplitR. { iPureIntro; constructor; auto with find_in_list. }
+            iPureIntro; aac_rewrite Heq; aac_reflexivity.
+          }
+          wp_pures.
+          wp_apply (push_buffer_element_spec with "[Hx Hpr2]") as "%pr3 #Hpr3". by iFrame "#".
+          wp_pures.
+          wp_apply (csref_alloc (fiveTuple depth (oX ++ oD)) with "[ι]") as "%ℓ' #Hℓ'". {
+            iExists pr3, ld', md, rd, sf,
+              (oX ++ o5), ((oX5 ++ oX6) ++ ldC), mdC, rdC, sfC,
+              5, 2, kSf.
+            iFrame "#".
+            iSplitR. done.
+            iSplitR. { iPureIntro; constructor; auto with find_in_list. }
+            iPureIntro; aac_rewrite Heq; aac_reflexivity.
+          }
+          wp_pures.
+          iApply "Hψ".
+          iFrame.
+          ℓisDeque ℓ'. iExact "Hℓ'".
+        * apply bool_decide_eq_false_1 in Heqb0 as prNotFull.
+          apply bool_decide_code_false in Heqb0 as ->.
+          wp_pures.
+          wp_bind (#ℓ <- _)%E.
+          wp_apply (csref_store with "[Hℓ]") as "_".
+          {
+            iSplitR. iExact "Hℓ".
+            iFrame. iExact "Hd".
+          }
+          wp_pures.
+          wp_apply (push_buffer_element_spec with "[Hpr Hx]") as "%pr' #Hpr'". by iFrame "#".
+          wp_pures.
+          wp_bind (ref _)%E.
+          wp_apply (csref_alloc (fiveTuple depth (oX ++ oD)) with "[ι]") as "%ℓ' #Hℓ'".
+          -- iExists pr', ld, md, rd, sf,
+              (oX ++ prC), ldC, mdC, rdC ,sfC,
+              (S kPr), kMd, kSf.
+            inversion cfg; [ exfalso; lia |].
+            iFrame "#".
+            iSplitR. done.
+            iSplitR. { iPureIntro; constructor; [invert_all_in | auto with find_in_list]. }
+            iPureIntro; aac_rewrite Heq; aac_reflexivity.
+          -- wp_pures.
+            iApply "Hψ".
+            iFrame.
+            ℓisDeque ℓ'.
+            iExact "Hℓ'".
+  Qed.
+
+  Theorem push_spec oD (x : val) (d : val) :
+    {{{ IsDeque oD d }}}
+      push x d
+    {{{ d', RET d'; IsDeque (⋅x ++ oD) d' }}}.
+  Proof.
+    iIntros (ψ) "HD Hψ".
+    rewrite /IsDeque.
+    wp_apply (push_spec_helper with "[HD]") as "%d' HD'".
+      { iFrame. rewrite /isElement. rewrite /=. iFrame. done. }
+    by iApply "Hψ".
+  Qed.
+
+  Corollary inject_spec_helper oD oX x d : forall depth,
+    {{{ isDeque depth oD d ∗ isElement depth oX x }}}
+      inject d x
+    {{{ d', RET d'; isDeque depth (oD ++ oX) d' }}}.
+ Admitted.
+
+  Corollary inject_spec oD (x : val) (d : val) :
+    {{{ IsDeque oD d }}}
+      inject d x
+    {{{ d', RET d'; IsDeque (oD ++ ⋅x) d' }}}.
+  Admitted.
+
+  (* NOTE(Juliette): Marked as 0 time cost, but runs in ⏱ (8 * time_for_push) constant time *)
+  Corollary push_whole_spec : forall lvl b oB d oD size,
+    {{{ buffer size lvl oB b ∗ isDeque lvl oD d }}}
+      push_whole_buffer push b d
+    {{{ d', RET d'; isDeque lvl (oB ++ oD) d' }}}.
+  Admitted.
+
+  (* NOTE(Juliette): Marked as 0 time cost, but runs in ⏱ (8 * time_for_push) constant time *)
+  Corollary inject_whole_spec : forall lvl b oB d oD size,
+    {{{ buffer size lvl oB b ∗ isDeque lvl oD d }}}
+      inject_whole_buffer inject d b
+    {{{ d', RET d'; isDeque lvl (oD ++ oB) d' }}}.
+  Admitted.
+
+  Lemma decrease_in : forall n o, n ∈ map S o -> ∃ k, n = S k ∧ k ∈ o.
+  Proof.
+    induction o; intros.
+    - inversion H.
+    - rewrite /= in H.
+      inversion H.
+      + exists a. split; auto with find_in_list.
+      + specialize (IHo H2) as (k & G1 & G2).
+        exists k. split; auto with find_in_list.
+  Qed.
+
+  Property partition_buffer_left_better_spec : forall lvl k o b,
+    {{{ buffer k lvl o b ∗ ⌜ k ∈ [2..6] ⌝ }}}
+      partition_buffer_left b
+    {{{ b1 b2 o1 o2 k1 k2, RET (b1, b2)%V;
+        buffer k1 lvl o1 b1 ∗ buffer k2 lvl o2 b2 ∗
+        ⌜ k1 ∈ [2; 3] ∧ k2 ∈ [0; 2; 3] ∧ o1 ++ o2 = o ⌝ }}}.
+  Proof.
+    destruct lvl.
+    - iIntros (k o b ψ) "[[#Hb <-] %Hk] Hψ".
+      wp_apply partition_buffer_left_spec as (b1 b2) "(%o1 & %o2 & Hb1 & Hb2 & (%Hl1 & %Hl2 & <-))".
+        by iFrame "#".
+      iApply "Hψ".
+      by iFrame.
+    - iIntros (k o b ψ) "[(%tr & %con & #Hb & (-> & <-) & Hall) %Hk] Hψ".
+      wp_apply partition_buffer_left_spec as (b1 b2) "(%o1 & %o2 & Hb1 & Hb2 & (%Hl1 & %Hl2 & <-))".
+        by iFrame "#".
+      iDestruct (big_sepL2_app_inv_l with "Hall") as "(%con1 & %con2 & %Heq & H1 & H2)".
+      iApply ("Hψ" $! b1 b2 (List.concat con1) (List.concat con2)).
+      iSplitL "Hb1 H1".
+        { iExists o1, con1. iFrame.
+          iSplitR. done.
+          iApply (big_sepL2_mono with "H1"); auto.
+        }
+      iSplitL.
+        { iExists o2, con2. iFrame.
+          iSplitR. done.
+          iApply (big_sepL2_mono with "H2"); auto.
+        }
+      iPureIntro.
+      do 2 (split; auto).
+      rewrite -concat_app -Heq //.
+  Qed.
+
+  Property partition_buffer_right_better_spec : forall lvl k o b,
+    {{{ buffer k lvl o b ∗ ⌜ k ∈ [2..6] ⌝ }}}
+      partition_buffer_right b
+    {{{ b1 b2 o1 o2 k1 k2, RET (b1, b2)%V;
+        buffer k1 lvl o1 b1 ∗ buffer k2 lvl o2 b2 ∗
+        ⌜ k1 ∈ [0; 2; 3] ∧ k2 ∈ [2; 3] ∧ o1 ++ o2 = o ⌝ }}}.
+  Admitted.
+
+  Theorem dconcat_spec (d1 d2 : val) : forall o1 o2,
+    {{{ IsDeque o1 d1 ∗ IsDeque o2 d2 }}}
+      dconcat d1 d2
+    {{{ d', RET d'; IsDeque (o1 ++ o2) d' }}}.
+  Proof.
+    iIntros (o1 o2 ψ) "(Hd1 & Hd2) Hψ".
+    iAssert emp%I as "ι". done. (* time cheat *)
+    rewrite /dconcat /IsDeque.
+    wp_pures.
+    wp_apply (tick_spec with "ι") as "_".
+    wp_pures.
+    (* trivial cases *)
+    rewrite {1} isDeque_unfold.
+    iDestruct "Hd1" as "[[-> ->] | (%ℓ1 & -> & #Hℓ1)]".
+    { wp_pures. iApply "Hψ". rewrite app_nil_l //. }
+    rewrite {1} isDeque_unfold.
+    iDestruct "Hd2" as "[[-> ->] | (%ℓ2 & -> & #Hℓ2)]".
+    { wp_pures. iApply "Hψ". iFrame. ℓisDeque ℓ1. rewrite app_nil_r. iExact "Hℓ1". }
+    wp_pures.
+    wp_apply (csref_load with "Hℓ1") as "%v
+      (%pr1 & %ld1 & %md1 & %rd1 & %sf1 & %oPr1 & %oLd1 & %oMd1 & %oRd1 & %oSf1 &
+      %kPr1 & %kMd1 & %kSf1 & -> & %cfg1 & #Hpr1 & #Hld1 & #Hmd1 & #Hrd1 & #Hsf1 & %Ho1)".
+    wp_pures.
+    wp_apply (bsize_better_spec with "Hmd1") as "_".
+    wp_pures.
+    destruct (bool_decide (kMd1 = 0)) eqn:?.
+    { (* d1 is suffix only *)
+      apply bool_decide_eq_true_1 in Heqb as Heqmd.
+      apply bool_decide_code_true in Heqb as ->.
+      wp_pures.
+      wp_apply (push_whole_spec) as "%d' #Hd'".
+        { iSplitR. iExact "Hsf1". iFrame. ℓisDeque ℓ2. iExact "Hℓ2". }
+      iApply "Hψ".
+      iFrame.
+      inversion cfg1; [| exfalso; lia].
+      iDestruct (empty_buffer_is_empty with "Hpr1") as "->".
+      iDestruct (empty_buffer_is_empty with "Hmd1") as "->".
+      rewrite (nil_length_inv _ (eq_sym H)) in Ho1 |- *.
+      rewrite (nil_length_inv _ (eq_sym H1)) in Ho1 |- *.
+      aac_normalise in Ho1.
+      rewrite Ho1 //.
+      }
+    apply bool_decide_eq_false_1 in Heqb as Heqmd1.
+    apply bool_decide_code_false in Heqb as ->.
+    wp_pures.
+    wp_apply (csref_load with "Hℓ2") as "%v'
+      (%pr2 & %ld2 & %md2 & %rd2 & %sf2 & %oPr2 & %oLd2 & %oMd2 & %oRd2 & %oSf2 &
+      %kPr2 & %kMd2 & %kSf2 & -> & %cfg2 & #Hpr2 & #Hld2 & #Hmd2 & #Hrd2 & #Hsf2 & %Ho2)".
+    wp_pures.
+    wp_apply (bsize_better_spec with "Hmd2") as "_".
+    wp_pures.
+    destruct (bool_decide (kMd2 = 0)) eqn:?.
+    { (* d2 is suffix only *)
+      apply bool_decide_eq_true_1 in Heqb as Heqmd.
+      apply bool_decide_code_true in Heqb as ->.
+      wp_pures.
+      wp_apply (inject_whole_spec) as "%d' #Hd'".
+        { iSplitR. iExact "Hsf2". iFrame. ℓisDeque ℓ1. iExact "Hℓ1". }
+      iApply "Hψ".
+      iFrame.
+      inversion cfg2; [| exfalso; by lia ].
+      iDestruct (empty_buffer_is_empty with "Hpr2") as "->".
+      iDestruct (empty_buffer_is_empty with "Hmd2") as "->".
+      rewrite (nil_length_inv _ (eq_sym H)) in Ho2 |- *.
+      rewrite (nil_length_inv _ (eq_sym H1)) in Ho2 |- *.
+      aac_normalise in Ho2.
+      rewrite Ho2 //.
+    }
+    apply bool_decide_eq_false_1 in Heqb as Heqmd2.
+    apply bool_decide_code_false in Heqb as ->.
+    wp_pures.
+    inversion cfg1; [exfalso; by apply Heqmd2 |].
+    inversion cfg2; [exfalso; by apply Heqmd2 |].
+    change (kPr2 ∈ map S [2; 3; 4; 5]) in H6.
+    apply decrease_in in H6 as (kPr2' & -> & HkPr2').
+    wp_apply (pop_buffer_element_spec with "Hpr2") as "%y %pr1' (%oY & %oBY & Hpr2' & -> & Hy)".
+    wp_pures.
+    change (kSf1 ∈ map S [2; 3; 4; 5]) in H0.
+    apply decrease_in in H0 as (kSf1' & -> & HkSf1').
+    wp_apply (eject_buffer_element_spec with "Hsf1") as "%sf1' %x (%oX & %oBX & Hsf1' & -> & Hx)".
+    wp_pures.
+    wp_apply (push_buffer_element_spec with "[Hy]") as "%bm Hbm".
+      { iFrame. by iApply empty_is_buffer_at. }
+    wp_apply (push_buffer_element_spec with "[Hbm Hx]") as "%md' #Hmd'". by iFrame.
+    wp_pures.
+    wp_apply (partition_buffer_left_better_spec with "[Hsf1']") as "%s1' %s1'' %os1' %os1'' %ks1' %ks1'' (#Hs1' & #Hs1'' & (%Hos1' & %Hos1'' & %Hos1eq))".
+      { iFrame. iPureIntro. invert_all_in. }
+    wp_pures.
+    rewrite !app_nil_r.
+    wp_apply (inject_spec_helper with "[Hld1]") as "%ld1' #Hld1'".
+      { iFrame "#". iFrame. rewrite /isElement triple_unfold.
+        iExists md1, rd1, s1', oMd1, oRd1, os1', kMd1, ks1'.
+        inversion cfg1; [ rewrite -H3 in H14; lia |].
+        iSplitR. iPureIntro.
+        destruct (length oRd1); [apply left_leaning | apply has_child];
+          auto with find_in_list arith.
+        iSplitR. done.
+        by iFrame "#".
+      }
+    wp_pures.
+    wp_bind (if: _ then _ else _)%E.
+    wp_apply (bsize_better_spec with "Hs1''") as "_".
+    wp_pures.
+    destruct (bool_decide (ks1'' = 0)) eqn:?.
+    + apply bool_decide_eq_true_1 in Heqb as Heqs1.
+      apply bool_decide_code_true in Heqb as ->.
+      wp_pures.
+      wp_apply (partition_buffer_right_better_spec with "[Hpr2']") as "%p2' %p2'' %op2' %op2'' %kp2' %kp2'' (#Hp2' & #Hp2'' & (%Hp21' & %Hp2'' & %Hop2eq))".
+        { iFrame. iPureIntro. invert_all_in. }
+      wp_pures.
+      wp_apply (push_spec_helper with "[Hrd2]") as "%rd2' #Hrd2'".
+      { iFrame "#". iFrame. rewrite /isElement triple_unfold.
+        iExists p2'', ld2, md2, op2'', oLd2, oMd2, kp2'', kMd2.
+        inversion cfg2.
+        iSplitR. iPureIntro.
+        destruct (length oLd2); [apply left_leaning | apply has_child];
+          auto with find_in_list arith.
+        iSplitR. done.
+        by iFrame "#".
+      }
+      wp_pures.
+      wp_bind (if: _ then _ else _)%E.
+      wp_apply (bsize_better_spec with "Hp2'") as "_".
+      wp_pures.
+      destruct (bool_decide (kp2' = 0)) eqn:?.
+      * apply bool_decide_eq_true_1 in Heqb as Heqp2.
+        apply bool_decide_code_true in Heqb as ->.
+        wp_pures.
+        wp_apply (csref_alloc (fiveTuple 0 (o1 ++ o2))) as (ℓ') "Hℓ'".
+          { iExists pr1, ld1', md', rd2', sf2,
+            oPr1, (oLd1 ++ oMd1 ++ oRd1 ++ os1'), (oX ++ oY), ((op2'' ++ oLd2 ++ oMd2) ++ oRd2), oSf2,
+            kPr1, 2, kSf2.
+            iSplitR. done.
+            iSplitR. iPureIntro. constructor; auto with find_in_list.
+            iFrame "#".
+            rewrite Heqs1 Heqp2.
+            iDestruct (empty_buffer_is_empty with "Hs1''") as "->".
+            iDestruct (empty_buffer_is_empty with "Hp2'") as "->".
+            iPureIntro.
+            rewrite Ho1 Ho2 -Hos1eq -Hop2eq.
+            aac_reflexivity.
+          }
+        wp_pures.
+        iApply "Hψ".
+        iFrame.
+        ℓisDeque ℓ'. iExact "Hℓ'".
+      * apply bool_decide_eq_false_1 in Heqb as Heqp2.
+        apply bool_decide_code_false in Heqb as ->.
+        wp_pures.
+        wp_apply (push_spec_helper with "[Hrd2']") as "%rd2'' #Hrd2''".
+          { iFrame "#". iFrame.
+            rewrite /isElement triple_unfold.
+            iExists p2', empty, empty_buffer, op2', [], [], kp2', 0.
+            iSplitR. iPureIntro. constructor; invert_all_in.
+            iSplitR. done.
+            iFrame "#".
+            iSplitR. isEmptyDeque.
+            iSplitR. rewrite /bufferPre. iSplitL. by iApply empty_is_buffer. done.
+            done.
+          }
+        wp_pures.
+        wp_apply (csref_alloc (fiveTuple 0 (o1 ++ o2))) as (ℓ') "Hℓ'".
+          { iExists pr1, ld1', md', rd2'', sf2,
+            oPr1, (oLd1 ++ oMd1 ++ oRd1 ++ os1'), (oX ++ oY), (op2' ++ (op2'' ++ oLd2 ++ oMd2) ++ oRd2), oSf2,
+            kPr1, 2, kSf2.
+            iSplitR. done.
+            iSplitR. iPureIntro. constructor; auto with find_in_list.
+            rewrite Heqs1 !app_nil_r.
+            iDestruct (empty_buffer_is_empty with "Hs1''") as "->".
+            iFrame "#".
+            iPureIntro.
+            rewrite Ho1 Ho2 -Hos1eq -Hop2eq.
+            aac_reflexivity.
+          }
+        wp_pures.
+        iApply "Hψ".
+        iFrame.
+        ℓisDeque ℓ'. iExact "Hℓ'".
+    + apply bool_decide_eq_false_1 in Heqb as Heqs1.
+      apply bool_decide_code_false in Heqb as ->.
+      wp_pures.
+        wp_apply (inject_spec_helper with "[Hld1']") as "%ld1'' #Hld1''".
+          { iFrame "#". iFrame.
+            rewrite /isElement triple_unfold.
+            iExists s1'', empty, empty_buffer, os1'', [], [], ks1'', 0.
+            iSplitR. iPureIntro. constructor; invert_all_in.
+            iSplitR. done.
+            iFrame "#".
+            iSplitR. isEmptyDeque.
+            iSplitR. rewrite /bufferPre. iSplitL. by iApply empty_is_buffer. done.
+            done.
+          }
+      wp_pures.
+      wp_apply (partition_buffer_right_better_spec with "[Hpr2']") as "%p2' %p2'' %op2' %op2'' %kp2' %kp2'' (#Hp2' & #Hp2'' & (%Hp21' & %Hp2'' & %Hop2eq))".
+        { iFrame. iPureIntro. invert_all_in. }
+      wp_pures.
+      wp_apply (push_spec_helper with "[Hrd2]") as "%rd2' #Hrd2'".
+      { iFrame "#". iFrame. rewrite /isElement triple_unfold.
+        iExists p2'', ld2, md2, op2'', oLd2, oMd2, kp2'', kMd2.
+        inversion cfg2.
+        iSplitR. iPureIntro.
+        destruct (length oLd2); [apply left_leaning | apply has_child];
+          auto with find_in_list arith.
+        iSplitR. done.
+        by iFrame "#".
+      }
+      wp_pures.
+      wp_bind (if: _ then _ else _)%E.
+      wp_apply (bsize_better_spec with "Hp2'") as "_".
+      wp_pures.
+      rewrite !app_nil_r.
+      destruct (bool_decide (kp2' = 0)) eqn:?.
+      * apply bool_decide_eq_true_1 in Heqb as Heqp2.
+        apply bool_decide_code_true in Heqb as ->.
+        wp_pures.
+        wp_apply (csref_alloc (fiveTuple 0 (o1 ++ o2))) as (ℓ') "Hℓ'".
+          { iExists pr1, ld1'', md', rd2', sf2,
+            oPr1, ((oLd1 ++ oMd1 ++ oRd1 ++ os1') ++ os1''), (oX ++ oY), ((op2'' ++ oLd2 ++ oMd2) ++ oRd2), oSf2,
+            kPr1, 2, kSf2.
+            iSplitR. done.
+            iSplitR. iPureIntro. constructor; auto with find_in_list.
+            iFrame "#".
+            rewrite Heqp2.
+            iDestruct (empty_buffer_is_empty with "Hp2'") as "->".
+            iPureIntro.
+            rewrite Ho1 Ho2 -Hos1eq -Hop2eq.
+            aac_reflexivity.
+          }
+        wp_pures.
+        iApply "Hψ".
+        iFrame.
+        ℓisDeque ℓ'. iExact "Hℓ'".
+      * apply bool_decide_eq_false_1 in Heqb as Heqp2.
+        apply bool_decide_code_false in Heqb as ->.
+        wp_pures.
+        wp_apply (push_spec_helper with "[Hrd2']") as "%rd2'' #Hrd2''".
+          { iFrame "#". iFrame.
+            rewrite /isElement triple_unfold.
+            iExists p2', empty, empty_buffer, op2', [], [], kp2', 0.
+            iSplitR. iPureIntro. constructor; invert_all_in.
+            iSplitR. done.
+            iFrame "#".
+            iSplitR. isEmptyDeque.
+            iSplitR. rewrite /bufferPre. iSplitL. by iApply empty_is_buffer. done.
+            done.
+          }
+        wp_pures.
+        wp_apply (csref_alloc (fiveTuple 0 (o1 ++ o2))) as (ℓ') "Hℓ'".
+          { iExists pr1, ld1'', md', rd2'', sf2,
+            oPr1, ((oLd1 ++ oMd1 ++ oRd1 ++ os1')++os1''), (oX ++ oY), (op2' ++ (op2'' ++ oLd2 ++ oMd2) ++ oRd2), oSf2,
+            kPr1, 2, kSf2.
+            iSplitR. done.
+            iSplitR. iPureIntro. constructor; auto with find_in_list.
+            rewrite !app_nil_r.
+            iFrame "#".
+            iPureIntro.
+            rewrite Ho1 Ho2 -Hos1eq -Hop2eq.
+            aac_reflexivity.
+          }
+        wp_pures.
+        iApply "Hψ".
+        iFrame.
+        ℓisDeque ℓ'. iExact "Hℓ'".
+  Qed.
+
+End proofs.
